tot_serialize_nlist_refine_eq

src/lowparse/LowParse.Spec.VCList.fst
@@ -159,3 +159,69 @@ let serialize_nlist
 = serialize_nlist' n s
 
 let tot_serialize_nlist n s = tot_serialize_nlist' n s
+
+#push-options "--z3rlimit 32"
+
+#restart-solver
+let rec tot_serialize_nlist_refine_eq
+  (#k: parser_kind)
+  (#t: Type)
+  (p: tot_parser k t { k.parser_kind_subkind == Some ParserStrong })
+  (f: t -> bool)
+  (fl: list t -> bool { forall l . fl l == List.Tot.for_all f l })
+  (s: tot_serializer (tot_parse_filter p f))
+  (n: nat)
+  (l: parse_filter_refine #(nlist n t) fl)
+: Lemma
+  (ensures (tot_serialize_nlist_refine p f fl s n l == tot_serialize_nlist_refine' p f fl s n l))
+  (decreases n)
+= refine_nlist_of_nlist_refine_injective f fl n;
+  refine_nlist_of_nlist_refine_inverse f fl n;
+  tot_serialize_synth_eq
+    (tot_parse_nlist n (tot_parse_filter p f))
+    (refine_nlist_of_nlist_refine f fl n)
+    (tot_serialize_nlist n s)
+    (nlist_refine_of_refine_nlist f fl n)
+    ()
+    l;
+  if n = 0
+  then ()
+  else begin
+    let a :: q = l in
+    let q : parse_filter_refine #(nlist (n - 1) t) fl = q in
+    tot_serialize_nlist_refine_eq p f fl s (n - 1) q;
+    refine_nlist_of_nlist_refine_injective f fl (n - 1);
+    refine_nlist_of_nlist_refine_inverse f fl (n - 1);
+    assert (refine_nlist_of_nlist_refine f fl (n - 1) (nlist_refine_of_refine_nlist f fl (n - 1) q) == q);
+    tot_serialize_nlist_cons (n - 1) s a (nlist_refine_of_refine_nlist f fl (n - 1) q);
+    assert (bare_serialize (tot_serialize_nlist (n - 1 + 1) s) (a :: nlist_refine_of_refine_nlist f fl (n - 1) q) == tot_serialize_nlist n s (nlist_refine_of_refine_nlist f fl n l));
+    assert (tot_serialize_nlist n s (nlist_refine_of_refine_nlist f fl n l) == s a `Seq.append` tot_serialize_nlist (n - 1) s (nlist_refine_of_refine_nlist f fl (n - 1) q));
+    assert (
+      tot_serialize_nlist_refine p f fl s (n - 1) q == tot_serialize_nlist_refine' p f fl s (n - 1) q
+    );
+    let _ : squash (
+      tot_serialize_nlist_refine p f fl s (n - 1) q == tot_serialize_nlist (n - 1) s (nlist_refine_of_refine_nlist f fl (n - 1) q)
+    ) =
+      assert_norm (
+        tot_serialize_nlist_refine p f fl s (n - 1) ==
+        tot_serialize_synth
+          (tot_parse_nlist (n - 1) (tot_parse_filter p f))
+          (refine_nlist_of_nlist_refine f fl (n - 1))
+          (tot_serialize_nlist (n - 1) s)
+          (nlist_refine_of_refine_nlist f fl (n - 1))
+          ()
+      );
+      tot_serialize_synth_eq
+        (tot_parse_nlist (n - 1) (tot_parse_filter p f))
+        (refine_nlist_of_nlist_refine f fl (n - 1))
+        (tot_serialize_nlist (n - 1) s)
+        (nlist_refine_of_refine_nlist f fl (n - 1))
+        ()
+        q
+    in
+    assert (
+      tot_serialize_nlist_refine p f fl s n l == tot_serialize_nlist_refine' p f fl s n l
+    )
+  end
+
+#pop-options
